pushing current work in Dirac.v; removed ket semantics from Quantum.v

Dirac.v
@@ -15,98 +15,229 @@ Notation "∣+⟩" := plus_state.
 Notation "∣-⟩" := minus_state.
 *)
 
-Notation "∣+⟩" := (/√2 .* ∣0⟩ .+ /√2 .* ∣1⟩).
-Notation "∣-⟩" := (/√2 .* ∣0⟩ .+ (-/√2) .* ∣1⟩).
+Notation "∣ + ⟩" := (/√2 .* ∣ 0 ⟩ .+ /√2 .* ∣ 1 ⟩).
+Notation "∣ - ⟩" := (/√2 .* ∣ 0 ⟩ .+ (-/√2) .* ∣ 1 ⟩).
 
 (* Hadamard properties *)
-Lemma H0_spec : hadamard × ∣0⟩ = ∣+⟩.
+Lemma H0_spec : hadamard × ∣ 0 ⟩ = ∣ + ⟩.
 Proof. solve_matrix. Qed.
 
-Lemma H1_spec : hadamard × ∣1⟩ = ∣-⟩.
+Lemma H1_spec : hadamard × ∣ 1 ⟩ = ∣ - ⟩.
 Proof. solve_matrix. Qed.
 
-Lemma Hplus_spec : hadamard × ∣+⟩ = ∣0⟩.
+Lemma Hplus_spec : hadamard × ∣ + ⟩ = ∣ 0 ⟩.
 Proof. solve_matrix. Qed.
 
-Lemma Hminus_spec : hadamard × ∣-⟩ = ∣1⟩.
+Lemma Hminus_spec : hadamard × ∣ - ⟩ = ∣ 1 ⟩.
 Proof. solve_matrix.  Qed.
 
 (* X properties *)
-Lemma X0_spec : σx × ∣0⟩ = ∣1⟩.
+Lemma X0_spec : σx × ∣ 0 ⟩ = ∣ 1 ⟩.
 Proof. solve_matrix. Qed.
 
-Lemma X1_spec : σx × ∣1⟩ = ∣0⟩.
+Lemma X1_spec : σx × ∣ 1 ⟩ = ∣ 0 ⟩.
 Proof. solve_matrix. Qed.
 
 (* Y properties *)
-Lemma Y0_spec : σy × ∣0⟩ = Ci .* ∣1⟩.
+Lemma Y0_spec : σy × ∣ 0 ⟩ = Ci .* ∣ 1 ⟩.
 Proof. solve_matrix. Qed.
 
-Lemma Y1_spec : σy × ∣1⟩ = -Ci .* ∣0⟩.
+Lemma Y1_spec : σy × ∣ 1 ⟩ = -Ci .* ∣ 0 ⟩.
 Proof. solve_matrix. Qed.
 
 (* Z properties *)
-Lemma Z0_spec : σz × ∣0⟩ = ∣0⟩.
+Lemma Z0_spec : σz × ∣ 0 ⟩ = ∣ 0 ⟩.
 Proof. solve_matrix. Qed.
 
-Lemma Z1_spec : σz × ∣1⟩ = -1 .* ∣1⟩.
+Lemma Z1_spec : σz × ∣ 1 ⟩ = -1 .* ∣ 1 ⟩.
 Proof. solve_matrix. Qed.
 
 (* CNOT properties *)
 
-Lemma CNOT_spec : forall (x y : nat), (x < 2)%nat -> (y < 2)%nat -> cnot × ∣x,y⟩ = ∣x, (x + y) mod 2⟩.
+Lemma CNOT_spec : forall (x y : nat), (x < 2)%nat -> (y < 2)%nat -> cnot × ∣ x,y ⟩ = ∣ x, (x + y) mod 2 ⟩.
 Proof.
   intros; destruct x as [| [|x]], y as [| [|y]]; try omega; solve_matrix.
 Qed.
 
-Lemma CNOT00_spec : cnot × ∣0,0⟩ = ∣0,0⟩.
+Lemma CNOT00_spec : cnot × ∣ 0,0 ⟩ = ∣ 0,0 ⟩.
 Proof. solve_matrix. Qed.
 
-Lemma CNOT01_spec : cnot × ∣0,1⟩ = ∣0,1⟩.
+Lemma CNOT01_spec : cnot × ∣ 0,1 ⟩ = ∣ 0,1 ⟩.
 Proof. crunch_matrix. Qed.
 
-Lemma CNOT10_spec : cnot × ∣1,0⟩ = ∣1,1⟩.
+Lemma CNOT10_spec : cnot × ∣ 1,0 ⟩ = ∣ 1,1 ⟩.
 Proof. solve_matrix. Qed.
                                         
-Lemma CNOT11_spec : cnot × ∣1,1⟩ = ∣1,0⟩.
+Lemma CNOT11_spec : cnot × ∣ 1,1 ⟩ = ∣ 1,0 ⟩.
 Proof. solve_matrix. Qed.
 
 (* SWAP properties *)
 
-Lemma SWAP_spec : forall x y, swap × ∣x,y⟩ = ∣y,x⟩.
+Lemma SWAP_spec : forall x y, swap × ∣ x,y ⟩ = ∣ y,x ⟩.
 Proof. intros. destruct x,y; solve_matrix. Qed.
 
 (* Automation *)
 
-Hint Rewrite Mmult_plus_distr_l Mscale_plus_distr Mscale_mult_dist_r Mscale_mult_dist_l : ket_db.
-Hint Rewrite Mscale_assoc Mmult_assoc: ket_db.
-Hint Rewrite Mscale_0_l Mscale_1_l : ket_db.
+(* General matrix rewrites *)
+Hint Rewrite Mmult_plus_distr_l Mmult_plus_distr_r kron_plus_distr_l kron_plus_distr_r Mscale_plus_distr_r : ket_db.
+Hint Rewrite Mscale_mult_dist_l Mscale_mult_dist_r Mscale_kron_dist_l Mscale_kron_dist_r : ket_db.
+Hint Rewrite Mscale_assoc Mmult_assoc : ket_db.
+(*Hint Rewrite <- Mplus_assoc kron_assoc : ket_db.*)
+Hint Rewrite Mmult_1_l Mmult_1_r kron_1_l kron_1_r Mscale_0_l Mscale_1_l Mplus_0_l Mplus_0_r : ket_db.
+Hint Rewrite kron_mixed_product.
+
+(* Quantum-specific identities *)
 Hint Rewrite H0_spec H1_spec Hplus_spec Hminus_spec X0_spec X1_spec Y0_spec Y1_spec
      Z0_spec Z1_spec : ket_db.
+Hint Rewrite CNOT00_spec CNOT01_spec CNOT10_spec CNOT11_spec SWAP_spec : ket_db.
+
+(* Examples using ket_db *)
+Lemma XYZ0 : -Ci .* σx × σy × σz × ∣ 0 ⟩ = ∣ 0 ⟩.
+Proof. autorewrite with ket_db C_db; easy. Qed.
+                                           
+Lemma XYZ1 : -Ci .* σx × σy × σz × ∣ 1 ⟩ = ∣ 1 ⟩.
+Proof. 
+  autorewrite with ket_db C_db. 
+  replace (Ci * -1 * Ci) with (RtoC 1) by clra. 
+  rewrite Mscale_1_l; reflexivity.
+  Qed.
+
+(* Simplify left-associated sums of terms of the form (a .* ∣ x ⟩).   
+   The end result should have the form (a .* ∣ 0 ⟩ .+ b .* ∣ 1 ⟩) *)
+Ltac simpl_ket_1_qubit :=
+  repeat
+  (match goal with
+    (* combine like terms *)
+    | [ |- context[ ?a .* ∣ ?x ⟩ .+ ?b .* ∣ ?x ⟩ ] ] => 
+          rewrite <- (Mscale_plus_distr_l _ _ a b ∣ x ⟩)
+    | [ |- context[ (?a .+ ?b .* ∣ ?x ⟩) .+ ?c .* ∣ ?x ⟩ ] ] => 
+          rewrite (Mplus_assoc _ _ a (b .* ∣ x ⟩) (c .* ∣ x ⟩));
+          rewrite <- (Mscale_plus_distr_l _ _ b c ∣ x ⟩)
+    (* reorder terms *)
+    | [ |- context[ ?a .* ∣ 1 ⟩ .+ ?b .* ∣ 0 ⟩ ] ] => 
+          rewrite (Mplus_comm _ _ (a .* ∣ 1 ⟩) (b .* ∣ 0 ⟩))
+    | [ |- context[ (?a .+ ?b .* ∣ 1 ⟩) .+ ?c .* ∣ 0 ⟩ ] ] => 
+          rewrite (Mplus_assoc _ _ a (b .* ∣ 1 ⟩) (c .* ∣ 0 ⟩));
+          rewrite (Mplus_comm _ _ (b .* ∣ 1 ⟩) (c .* ∣ 0 ⟩)); 
+          rewrite <- (Mplus_assoc _ _ a (c .* ∣ 0 ⟩) (b .* ∣ 1 ⟩))
+   
+  end).
+    
+(* Simplify left-associated sums of terms of the form (a .* ∣ x,y ⟩).
+   The end result should have the form
+       a .* ∣ 0,0 ⟩ .+ b .* ∣ 0,1 ⟩ .+ c .* ∣ 1,0 ⟩ .+ d .* ∣ 1,1 ⟩ *)
+Open Scope nat_scope.
+Ltac simpl_ket_2_qubit :=
+  repeat
+  (match goal with
+    (* combine like terms *)
+    | [ |- context[ ?a .* ∣ ?x,?y ⟩ .+ ?b .* ∣ ?x,?y ⟩ ] ] => 
+          rewrite <- (Mscale_plus_distr_l _ _ a b ∣ x,y ⟩)
+    | [ |- context[ (?a .+ ?b .* ∣ ?x,?y ⟩) .+ ?c .* ∣ ?x,?y ⟩ ] ] => 
+          rewrite (Mplus_assoc _ _ a (b .* ∣ x,y ⟩) (c .* ∣ x,y ⟩));
+          rewrite <- (Mscale_plus_distr_l _ _ b c ∣ x,y ⟩)
+    (* reorder terms *)
+    (* NOTE: we could also write explicit rules for 00, 01, 10, 11,
+       but this seemed cleaner. I don't know how this style impacts
+       automation efficiency. *) 
+    | [ |- context[ ?a .* ∣ ?x,?y ⟩ .+ ?b .* ∣ ?x',?y' ⟩ ] ] => 
+          assert ((x' < x) \/ (x' = x /\ y' < y)) by omega;
+          rewrite (Mplus_comm _ _ (a .* ∣ x,y ⟩) (b .* ∣ x',y' ⟩))
+    | [ |- context[ ?a .+ ?b .* ∣ ?x,?y ⟩ .+ ?c .* ∣ ?x',?y' ⟩ ] ] => 
+          assert ((x' < x) \/ (x' = x /\ y' < y)) by omega;
+          rewrite (Mplus_assoc _ _ a (b .* ∣ x,y ⟩) (c .* ∣ x',y' ⟩));
+          rewrite (Mplus_comm _ _ (b .* ∣ x,y ⟩) (c .* ∣ x',y' ⟩)); 
+          rewrite <- (Mplus_assoc _ _ a (c .* ∣ x',y' ⟩) (b .* ∣ x,y ⟩))   
+  end). 
+Close Scope nat_scope. 
+
+(* The main issue with simpl_ket_1_qubit and simpl_ket_2_qubit is that
+   they expect the goal to be in a particular form, so I need to write
+   additional tactics to put the goal in the desired form.
+
+   I'd also like to write a version of ket_eq_solver that works for
+   multi-qubit systems. *)
 
 Ltac ket_eq_solver :=
   intros; autorewrite with ket_db C_db;
   try match goal with
-  | [|- ?a .* ∣0⟩ .+ ?b .* ∣1⟩ = ?a' .* ∣0⟩ .+ ?b' .* ∣1⟩ ] =>
-    replace a with a'; try clra; replace b with b'; try clra; trivial
-  end.                                                           
+  | [ |- ?a .* ∣ 0 ⟩ .+ ?b .* ∣ 1 ⟩ = ?a' .* ∣ 0 ⟩ .+ ?b' .* ∣ 1 ⟩ ] =>
+    replace a with a' by clra; replace b with b' by clra; reflexivity
+  end.      
 
-Lemma XYZ0 : -Ci .* σx × σy × σz × ∣0⟩ = ∣0⟩.
-Proof. autorewrite with ket_db C_db; easy. Qed.
-                                            
-Lemma XYZ1 : -Ci .* σx × σy × σz × ∣1⟩ = ∣1⟩.
-Proof. autorewrite with ket_db C_db; easy. Qed.
-
-Lemma XYZ : forall α β, -Ci .* σx × σy × σz × (α .* ∣0⟩ .+ β .* ∣1⟩) = α .* ∣0⟩ .+ β .* ∣1⟩.
+Lemma XYZ : forall α β, -Ci .* σx × σy × σz × (α .* ∣ 0 ⟩ .+ β .* ∣ 1 ⟩) = α .* ∣ 0 ⟩ .+ β .* ∣ 1 ⟩.
 Proof. ket_eq_solver. Qed.
 
+(* This proof would be nicest with +/- basis specific rewriting.
+
 Proposition HZH : forall α β,
-  hadamard × σz × hadamard × (α .* ∣0⟩ .+ β .* ∣1⟩) = σx × (α .* ∣0⟩ .+ β .* ∣1⟩).
+  hadamard × σz × hadamard × (α .* ∣ 0 ⟩ .+ β .* ∣ 1 ⟩) = σx × (α .* ∣ 0 ⟩ .+ β .* ∣ 1 ⟩).
 Proof.
   ket_eq_solver.
 Abort.
-
-(* Next up:
-   Multiqubit systems.
-   Have ket_eq_solver group ∣0⟩s and ∣1⟩s.
 *)
+
+
+(* Unitary superdense coding example (in-progress *)
+
+Require Import SQIMP.
+Require Import UnitarySem.
+Open Scope ucom_scope.
+
+Definition a : Var := O.
+Definition b : Var := S O.
+
+Definition bell00_u : ucom :=
+    a *= _H;
+    [a,b] *= CNOT.
+
+Definition encode_u (b1 b2 : bool): ucom :=
+    (if b2 then a *= _X else uskip);
+    (if b1 then a *= _Z else uskip).
+
+Definition decode_u : ucom := (* note: this is the reverse of bell00 *)
+    [a,b] *= CNOT;
+    a *= _H.
+
+Definition superdense_u (b1 b2 : bool) := bell00_u ; encode_u b1 b2; decode_u.
+
+Close Scope ucom_scope.
+
+(* Rewriting seems to be more cooperative with this definition of 
+   kron_mixed_product *)
+Lemma kron_mixed_prod2: forall (A : Matrix 2 2) (B : Matrix 2 2) x y,
+    (A ⊗ B) × ∣ x,y ⟩ = (A × ∣ x ⟩) ⊗ (B × ∣ y ⟩).
+Proof. intros. rewrite kron_mixed_product. reflexivity. Qed.
+Hint Rewrite kron_mixed_prod2 : ket_db.
+
+(*Set Printing All.*)
+Lemma superdense_correct : forall b1 b2, (uc_eval 2 (superdense_u b1 b2)) × ∣ 0,0 ⟩ = ∣ if b1 then S O else O,if b2 then S O else O ⟩.
+Proof.
+  intros; simpl.
+  replace (denote_ctrls 2 CNOT [a, b]) with cnot.
+  2: { unfold denote_ctrls. simpl. solve_matrix. }
+  destruct b1; destruct b2; simpl.
+  - autorewrite with ket_db C_db; try show_wf.
+    replace (Init.Nat.mul (S (S O)) (S (S O))) with (S (S (S (S O)))) by easy.
+    autorewrite with ket_db C_db; try show_wf.
+    replace (Init.Nat.mul (S (S O)) (S (S O))) with (S (S (S (S O)))) by easy.
+    autorewrite with ket_db C_db; try show_wf.
+    (* need to use coqeulicot tactics to prove this *)
+    replace (Cmult (Cmult (Cinv (RtoC (sqrt (IZR (Zpos (xO xH))))))
+                          (RtoC (IZR (Zneg xH)))) 
+                   (Cinv (RtoC (sqrt (IZR (Zpos (xO xH))))))) 
+      with (Copp (Cinv (RtoC (IZR (Zpos (xO xH)))))) by admit.
+    repeat (rewrite <- Mplus_assoc).
+    replace (S (S (S (S O)))) with (Init.Nat.mul (S (S O)) (S (S O))) by easy.
+    simpl_ket_2_qubit.
+    autorewrite with ket_db C_db.
+    reflexivity.
+  - autorewrite with ket_db C_db; try show_wf.
+    replace (Init.Nat.mul (S (S O)) (S (S O))) with (S (S (S (S O)))) by easy.
+    autorewrite with ket_db C_db; try show_wf.
+    replace (Init.Nat.mul (S (S O)) (S (S O))) with (S (S (S (S O)))) by easy.
+    autorewrite with ket_db C_db; try show_wf.
+Abort.
+                                                                             
+
+
